theories/examples/future_fibonacci__code.v
@@ -11,20 +11,25 @@ From examples Require Import
 From zoo Require Import
   options.
 
-Definition future_fibonacci_fibonacci_0 : val :=
-  rec: "fibonacci" "n" "ctx" =>
+Definition future_fibonacci_main_0 : val :=
+  rec: "main" "ctx" "n" =>
     if: "n" ≤ 1 then (
       "n"
     ) else (
       let: "fut1" :=
-        future_async "ctx" (fun: "ctx" => "fibonacci" ("n" - 1) "ctx")
+        future_async "ctx" (fun: "ctx" => "main" "ctx" ("n" - 1))
       in
       let: "fut2" :=
-        future_async "ctx" (fun: "ctx" => "fibonacci" ("n" - 2) "ctx")
+        future_async "ctx" (fun: "ctx" => "main" "ctx" ("n" - 2))
       in
       future_wait "ctx" "fut1" + future_wait "ctx" "fut2"
     ).
 
-Definition future_fibonacci_fibonacci : val :=
-  fun: "n" "pool" =>
-    pool_run "pool" (fun: "ctx" => future_fibonacci_fibonacci_0 "n" "ctx").
+Definition future_fibonacci_main : val :=
+  fun: "num_dom" "n" =>
+    let: "pool" := pool_create "num_dom" in
+    let: "res" :=
+      pool_run "pool" (fun: "ctx" => future_fibonacci_main_0 "ctx" "n")
+    in
+    pool_kill "pool" ;;
+    "res".
