theories/examples/future_fibonacci__opaque.v
@@ -1,4 +1,4 @@
 From examples Require Import
   future_fibonacci__code.
 
-#[global] Opaque future_fibonacci_fibonacci.
+#[global] Opaque future_fibonacci_main.
